Foundation/Modal/Hilbert/Minimal/Basic.lean
@@ -103,6 +103,9 @@ section
 
 abbrev logic (H : Hilbert.WithRE α) : Logic α := Entailment.theory H
 
+@[simp high]
+lemma iff_logic_provable_provable : H.logic ⊢! φ ↔ H ⊢! φ := by simp [Entailment.theory, Logic.iff_provable];
+
 instance [H₁ ⪯ H₂] : H₁.logic ⪯ H₂.logic := by
   apply weakerThan_iff.mpr;
   simp only [theory, Logic.iff_provable, Set.mem_setOf_eq];
